Introduce pborrow_deriv to examples.logic

nola/examples/logic.v
@@ -1,23 +1,38 @@
 (** * Showcase logic *)
 
-From nola.iris Require Export ciprop inv_deriv.
+From nola.iris Require Export ciprop inv_deriv pborrow_deriv.
 From nola.bi Require Import util.
 From nola.heap_lang Require Export notation proofmode lib.mutex.
-Import WpwNotation iPropAppNotation PintpNotation IntpNotation.
+From nola.examples Require Export nsynty.
+Import ProdNotation WpwNotation iPropAppNotation PintpNotation IntpNotation
+  NsyntyNotation.
 
-Implicit Type (N : namespace) (l : loc) (b : bool).
+Implicit Type (N : namespace) (l : loc) (b : bool) (α : lft) (q : Qp)
+  (X Y : nsynty).
 
 (** ** Preliminaries *)
 
 (** [sel]: Selector *)
 Variant sel :=
 | (** Invariant *) cips_inv (N : namespace)
-| (** Mutex *) cips_mutex (l : loc).
+| (** Mutex *) cips_mutex (l : loc)
+| (** Non-prophetic closed borrower *) cips_borc (α : lft)
+| (** Non-prophetic borrower *) cips_bor (α : lft)
+| (** Non-prophetic open borrower *) cips_obor (α : lft) (q : Qp)
+| (** Non-prophetic lender *) cips_lend (α : lft)
+| (** Prophetic closed borrower *)
+    cips_pborc {X} (α : lft) (x : X) (ξ : prvar X)
+| (** Prophetic borrower *) cips_pbor {X} (α : lft) (x : X) (ξ : prvar X)
+| (** Prophetic open borrower *) cips_pobor {X} (α : lft) (q : Qp) (ξ : prvar X)
+| (** Prophetic lender *) cips_plend {X} (α : lft) (xπ : clair nsynty X).
 (** [idom]: Domain for inductive parts *)
 Definition idom (_ : sel) : Type := Empty_set.
 (** [cdom]: Domain for coinductive parts *)
 Definition cdom (s : sel) : Type := match s with
-  | cips_inv _ | cips_mutex _ => unit
+  | cips_inv _ | cips_mutex _
+    | cips_borc _ | cips_bor _ | cips_obor _ _ | cips_lend _ => unit
+  | @cips_pborc X _ _ _ | @cips_pbor X _ _ _ | @cips_pobor X _ _ _
+    | @cips_plend X _ _ => X
   end.
 (** [dataOF]: Data [oFunctor] *)
 Definition dataOF (_ : sel) : oFunctor := unitO.
@@ -37,34 +52,94 @@ Proof. exact _. Qed.
 Section ciProp.
   Context {Σ : gFunctors}.
   Implicit Type Px : ciProp Σ.
+  (** Invariant *)
   Definition cip_inv N Px : ciProp Σ :=
     cip_custom (cips_inv N) nullary (unary Px) ().
+  (** Mutex *)
   Definition cip_mutex l Px : ciProp Σ :=
     cip_custom (cips_mutex l) nullary (unary Px) ().
+  (** Non-prophetic closed borrower *)
+  Definition cip_borc α Px : ciProp Σ :=
+    cip_custom (cips_borc α) nullary (unary Px) ().
+  (** Non-prophetic borrower *)
+  Definition cip_bor α Px : ciProp Σ :=
+    cip_custom (cips_bor α) nullary (unary Px) ().
+  (** Non-prophetic open borrower *)
+  Definition cip_obor α q Px : ciProp Σ :=
+    cip_custom (cips_obor α q) nullary (unary Px) ().
+  (** Non-prophetic lender *)
+  Definition cip_lend α Px : ciProp Σ :=
+    cip_custom (cips_lend α) nullary (unary Px) ().
+  (** Prophetic closed borrower *)
+  Definition cip_pborc {X} α x ξ (Φx : X -d> ciProp Σ) : ciProp Σ :=
+    cip_custom (@cips_pborc X α x ξ) nullary Φx ().
+  (** Prophetic borrower *)
+  Definition cip_pbor {X} α x ξ (Φx : X -d> ciProp Σ) : ciProp Σ :=
+    cip_custom (@cips_pbor X α x ξ) nullary Φx ().
+  (** Prophetic open borrower *)
+  Definition cip_pobor {X} α q ξ (Φx : X -d> ciProp Σ) : ciProp Σ :=
+    cip_custom (@cips_pobor X α q ξ) nullary Φx ().
+  (** Prophetic lender *)
+  Definition cip_plend {X} α xπ (Φx : X -d> ciProp Σ) : ciProp Σ :=
+    cip_custom (@cips_plend X α xπ) nullary Φx ().
 
+  (** The custom constructors are non-expansive *)
   #[export] Instance cip_inv_ne {N} : NonExpansive (cip_inv N).
   Proof. move=> ????. apply cip_custom_ne; solve_proper. Qed.
   #[export] Instance cip_mutex_ne {l} : NonExpansive (cip_mutex l).
+  Proof. move=> ????. apply cip_custom_ne; solve_proper. Qed.
+  #[export] Instance cip_borc_ne {α} : NonExpansive (cip_borc α).
+  Proof. move=> ????. apply cip_custom_ne; solve_proper. Qed.
+  #[export] Instance cip_bor_ne {α} : NonExpansive (cip_bor α).
+  Proof. move=> ????. apply cip_custom_ne; solve_proper. Qed.
+  #[export] Instance cip_obor_ne {α q} : NonExpansive (cip_obor α q).
+  Proof. move=> ????. apply cip_custom_ne; solve_proper. Qed.
+  #[export] Instance cip_lend_ne {α} : NonExpansive (cip_lend α).
+  Proof. move=> ????. apply cip_custom_ne; solve_proper. Qed.
+  #[export] Instance cip_pborc_ne {X α x ξ} : NonExpansive (@cip_pborc X α x ξ).
+  Proof. move=> ????. apply cip_custom_ne; solve_proper. Qed.
+  #[export] Instance cip_pbor_ne {X α x ξ} : NonExpansive (@cip_pbor X α x ξ).
+  Proof. move=> ????. apply cip_custom_ne; solve_proper. Qed.
+  #[export] Instance cip_pobor_ne {X α q ξ} : NonExpansive (@cip_pobor X α q ξ).
+  Proof. move=> ????. apply cip_custom_ne; solve_proper. Qed.
+  #[export] Instance cip_plend_ne {X α xπ} : NonExpansive (@cip_plend X α xπ).
   Proof. move=> ????. apply cip_custom_ne; solve_proper. Qed.
 End ciProp.
 
 (** ** [judg]: Judgment *)
 Definition judg Σ : ofe :=
-  (leibnizO namespace * ciProp Σ + ciProp Σ * ciProp Σ)%type.
-Definition inv_jacsr {Σ} N Px : judg Σ := inl (N, Px).
-Definition mutex_jiff {Σ} Px Qx : judg Σ := inr (Px, Qx).
+  (leibnizO namespace * ciProp Σ + ciProp Σ * ciProp Σ + ciProp Σ * ciProp Σ +
+    sigT (A:=nsynty *' nsynty) (λ '(X, Y)',
+      leibnizO (clair nsynty X *' clair nsynty Y) *
+      (X -d> ciProp Σ) * (Y -d> ciProp Σ)))%type.
+Definition inv_jacsr {Σ} N Px : judg Σ := inl (inl (inl (N, Px))).
+Definition mutex_jiff {Σ} Px Qx : judg Σ := inl (inl (inr (Px, Qx))).
+Definition pborrow_jto {Σ} Px Qx : judg Σ := inl (inr (Px, Qx)).
+Definition pborrow_jlto {Σ X Y} xπ yπ Φx Ψx : judg Σ :=
+  inr (existT (X, Y)' ((xπ, yπ)', Φx, Ψx)).
 #[export] Instance inv_jacsr_ne {Σ N} : NonExpansive (@inv_jacsr Σ N).
-Proof. move=> ????. exact: inl_ne. Qed.
+Proof. move=> ????. by do 3 apply: inl_ne. Qed.
 #[export] Instance mutex_jiff_ne {Σ} : NonExpansive2 (@mutex_jiff Σ).
-Proof. move=> ???????. exact: inr_ne. Qed.
+Proof. move=> ???????. do 2 apply: inl_ne. exact: inr_ne. Qed.
+#[export] Instance pborrow_jto_ne {Σ} : NonExpansive2 (@pborrow_jto Σ).
+Proof. move=> ???????. apply: inl_ne. exact: inr_ne. Qed.
+#[export] Instance pborrow_jlto_ne {Σ X Y xπ yπ} :
+  NonExpansive2 (@pborrow_jlto Σ X Y xπ yπ).
+Proof.
+  move=> ???????. apply inr_ne. apply: existT_ne=>/=. by split; [split|].
+Qed.
 
 #[export] Instance judg_inv_pre_deriv {Σ} :
   InvPreDeriv (ciProp Σ) (judg Σ) := INV_PRE_DERIV inv_jacsr.
 #[export] Instance judg_mutex_pre_deriv {Σ} :
   MutexPreDeriv (ciProp Σ) (judg Σ) := MUTEX_PRE_DERIV mutex_jiff.
+#[export] Instance judg_pborrow_pre_deriv {Σ} :
+  PborrowPreDeriv nsynty (ciProp Σ) (judg Σ) :=
+  PBORROW_PRE_DERIV pborrow_jto (@pborrow_jlto _).
 
 Section intp.
-  Context `{!inv'GS ciPropOF Σ, !mutexGS ciPropOF Σ}.
+  Context `{!inv'GS ciPropOF Σ, !mutexGS ciPropOF Σ,
+    !pborrowGS nsynty ciPropOF Σ}.
   Implicit Type δ : judg Σ → iProp Σ.
 
   (** ** [bintp]: Base interpretation *)
@@ -73,6 +148,14 @@ Section intp.
     match s with
     | cips_inv N => λ _ Pxs _, inv' δ N (Pxs ())
     | cips_mutex l => λ _ Pxs _, mutex δ l (Pxs ())
+    | cips_borc α => λ _ Pxs _, nborc δ α (Pxs ())
+    | cips_bor α => λ _ Pxs _, nbor δ α (Pxs ())
+    | cips_obor α q => λ _ Pxs _, nobor δ α q (Pxs ())
+    | cips_lend α => λ _ Pxs _, nlend δ α (Pxs ())
+    | cips_pborc α x ξ => λ _ Φx _, pborc δ α x ξ Φx
+    | cips_pbor α x ξ => λ _ Φx _, pbor δ α x ξ Φx
+    | cips_pobor α q ξ => λ _ Φx _, pobor δ α q ξ Φx
+    | cips_plend α xπ => λ _ Φx _, plend δ α xπ Φx
     end.
 
   (** [bintp] is non-expansive *)
@@ -92,12 +175,20 @@ Section intp.
 
   (** [judg_intp]: Judgment interpretation *)
   Definition judg_intp δ (J : judg Σ) := match J with
-    | inl (N, Px) => inv_acsr ⟦⟧(δ) N ⟦ Px ⟧(δ)
-    | inr (Px, Qx) => mod_iff (fupd ⊤ ⊤) ⟦ Px ⟧(δ) ⟦ Qx ⟧(δ)
+    | inl (inl (inl (N, Px))) => inv_acsr ⟦⟧(δ) N ⟦ Px ⟧(δ)
+    | inl (inl (inr (Px, Qx))) => mod_iff (fupd ⊤ ⊤) ⟦ Px ⟧(δ) ⟦ Qx ⟧(δ)
+    | inl (inr (Px, Qx)) => ⟦ Px ⟧(δ) ==∗ ⟦ Qx ⟧(δ)
+    | inr (existT (X, Y)' ((xπ, yπ)', Φx, Ψx)) =>
+        plend_body ⟦ ⟧(δ) xπ Φx ==∗ plend_body ⟦ ⟧(δ) yπ Ψx
     end%I.
   Local Instance judg_intp_ne `{!NonExpansive δ} : NonExpansive (judg_intp δ).
   Proof.
-    move=> ???[[??][??][/=/leibniz_equiv_iff-> ?]|[??][??][/=??]]; solve_proper.
+    move=> ? _ _[_ _[_ _[|]|]|].
+    - move=> [??][??][/=/leibniz_equiv_iff<- ?]. solve_proper.
+    - move=> [??][??][/=??]. solve_proper.
+    - move=> [??][??]/=[??]. solve_proper.
+    - move=> [?[[[??]?]?]][?[[[??]?]?]][/=?]. subst=>/=.
+      move=> [/=[/=/leibniz_equiv_iff[<-<-]?]?]. solve_proper.
   Qed.
   #[export] Instance judg_dintp : Dintp (judg Σ) (judg Σ) (iProp Σ) :=
     DINTP judg_intp.
@@ -106,6 +197,8 @@ Section intp.
   #[export] Instance judg_inv_deriv : InvDeriv ciPropOF Σ judgJ.
   Proof. done. Qed.
   #[export] Instance judg_mutex_deriv : MutexDeriv ciPropOF Σ judgJ.
+  Proof. done. Qed.
+  #[export] Instance judg_pborrow_deriv : PborrowDeriv nsynty ciPropOF Σ judgJ.
   Proof. done. Qed.
 End intp.
 
@@ -117,7 +210,8 @@ Definition iter_ilist : val := rec: "self" "f" "c" "l" :=
     "f" "l";; "c" <- !"c" - #1;; "self" "f" "c" (!("l" +ₗ #1)).
 
 Section verify.
-  Context `{!inv'GS ciPropOF Σ, !mutexGS ciPropOF Σ, !heapGS_gen hlc Σ}.
+  Context `{!inv'GS ciPropOF Σ, !mutexGS ciPropOF Σ,
+    !pborrowGS nsynty ciPropOF Σ, !heapGS_gen hlc Σ}.
   Implicit Type Φx Ψx : loc → ciProp Σ.
 
   (** [ilist]: Syntactic proposition for a list *)
@@ -194,7 +288,8 @@ Definition iter_mlist : val := rec: "self" "f" "k" "c" "l" :=
     else #false.
 
 Section verify.
-  Context `{!inv'GS ciPropOF Σ, !mutexGS ciPropOF Σ, !heapGS_gen hlc Σ}.
+  Context `{!inv'GS ciPropOF Σ, !mutexGS ciPropOF Σ,
+    !pborrowGS nsynty ciPropOF Σ, !heapGS_gen hlc Σ}.
   Implicit Type Φx : loc → ciProp Σ.
 
   (** [mlist]: Syntactic proposition for a list with a mutex *)
